more Hoare stuff for dealing with framing/splitting hopefully

Hoare/Hoare_Lift.thy
@@ -76,12 +76,11 @@ definition lift_pred_valid_s ::
 definition lift_pred_validx_s ::
   "('a1, 'b1) syn_lifting \<Rightarrow>
    ('a1, 'a2, 'b2 :: {Pord, Okay}, 'z) lifting_scheme \<Rightarrow>
-   ('a1 \<Rightarrow> 'b2 set) \<Rightarrow>
    'b1 \<Rightarrow>
    ('a2 \<Rightarrow> bool) \<Rightarrow>
    ('b2 \<Rightarrow> bool)"
   where
-"lift_pred_validx_s l' l S syn P st =
+"lift_pred_validx_s l' l syn P st =
   (lift_pred_s l' l syn P st \<and> st \<in> ok_S)" 
 
 lemma Vlift_valid' :
@@ -98,7 +97,7 @@ lemma Vlift_validx' :
   assumes Validx : "lifting_validx l S" 
   assumes V: "(sem) % {{P}} x {{Q}}"
   assumes Syn : "l' x' = x"
-  shows "(lift_map_s l' l sem) % {{lift_pred_validx_s l' l S x' P}} x' {{lift_pred_validx_s l' l S x' Q}}"
+  shows "(lift_map_s l' l sem) % {{lift_pred_validx_s l' l x' P}} x' {{lift_pred_validx_s l' l  x' Q}}"
  using V Syn
   unfolding HTS_def HT_def lift_pred_s_def lift_map_s_def lift_pred_valid_s_def lift_pred_validx_s_def
   using lifting_validDP[OF lifting_validxDV[OF Validx]] lifting_validxDP'[OF Validx]
