Hoare/Hoare_Step.thy
@@ -3,7 +3,7 @@ theory Hoare_Step imports Hoare Hoare_Indexed Hoare_Direct
  "../Mergeable/Mergeable_Instances"
  "../Composition/Composition" "../Composition/Dominant"
  "../Language_Components/Seq/Seq_Hoare"
- "Hoare_Lift"
+ "Hoare_Lift" "Hoare_Lift_Transform"
 begin
 
 (* 
@@ -80,26 +80,26 @@ lemma HTS_imp_HT' :
   assumes Skip : "lfts c = Sskip"
   assumes Hnemp : "g \<in> (set fs - {seq_sem_l_gen lfts})"
   assumes Hdom : "(f' \<downharpoonleft> (set fs - {seq_sem_l_gen lfts}) c)"
-  shows "|gs| {~ (lift_pred_validx_s id l S c P1) ~} [G c z] {~ (lift_pred_validx_s id l S c P2) ~}"
+  shows "|gs| {~ (lift_pred_validx_s id l c P1) ~} [G c z] {~ (lift_pred_validx_s id l c P2) ~}"
 proof(rule HT'I)
   fix npost
 
   have Valid' : "lifting_valid l S"
     using lifting_validxDV[OF Valid] by auto
 
-  have "|#gs#| {#-lift_pred_validx_s id l S c
+  have "|#gs#| {#-lift_pred_validx_s id l c
                      P1, (0 +
-                          npost)-#} [G c z] {#-lift_pred_validx_s id l S c
+                          npost)-#} [G c z] {#-lift_pred_validx_s id l c
        P2, npost-#}"
     unfolding add_0
   proof
     fix c'
 
-    assume Guard : "|#gs#| {#lift_pred_validx_s id l S c P2, npost#} c'"
-    show "|#gs#| {#lift_pred_validx_s id l S c P1, npost#} ([G c z] @ c')"
+    assume Guard : "|#gs#| {#lift_pred_validx_s id l c P2, npost#} c'"
+    show "|#gs#| {#lift_pred_validx_s id l c P1, npost#} ([G c z] @ c')"
     proof
       fix m :: "('a, 'c) control"
-      assume Hpay : "lift_pred_validx_s id l S c P1 (payload m)"
+      assume Hpay : "lift_pred_validx_s id l c P1 (payload m)"
       assume Hcont : "cont m = Inl ([G c z] @ c') "
 
       have Hpay1 : "P1 (LOut l c (payload m))" and Hpay2 : "payload m \<in> S c" and Hpay3 : "payload m \<in> ok_S"
@@ -273,10 +273,269 @@ proof(rule HT'I)
   qed
 
   thus "\<exists>npre.
-          |#gs#| {#-lift_pred_validx_s id l S c
-                     P1, (npre + npost)-#} [G c z] {#-lift_pred_validx_s id l S c P2, npost-#}"
+          |#gs#| {#-lift_pred_validx_s id l c
+                     P1, (npre + npost)-#} [G c z] {#-lift_pred_validx_s id l c P2, npost-#}"
     by blast
 qed
+
+(* TODO: there is a spurious Pord constraint on f for some reason. *)
+lemma HTS_imp_HT'' :
+  assumes H: "\<And> P1 . f % {{P1}} c {{P2 P1}}"
+  assumes Valid : "lifting_validx l S"
+  assumes Hf' : "f' = no_control_l l f"
+  assumes H0 : "gs = pcomps fs"
+  assumes Hpres : "sups_pres (set fs)"
+  assumes Hseq : "seq_sem_l_gen lfts \<in> set fs"
+  assumes Skip : "lfts c = Sskip"
+  assumes Hnemp : "g \<in> (set fs - {seq_sem_l_gen lfts})"
+  assumes Hdom : "(f' \<downharpoonleft> (set fs - {seq_sem_l_gen lfts}) c)"
+  assumes P1_ok : "\<And> st . P1 st \<Longrightarrow> st \<in> ok_S"
+  shows "|gs| {~ (\<lambda> st . P1 st) ~} [G c z] {~ (\<lambda> st . liftt_conc id l c P2 P1 st) ~}"
+  (*shows "\<And> P1 . |gs| {~ P1 ~} [G c z] {~ (liftt_conc id l c P2 P1) ~}"*)
+proof(rule HT'I)
+  fix npost
+
+  have Valid' : "lifting_valid l S"
+    using lifting_validxDV[OF Valid] by auto
+
+  have "|#gs#| {#-(\<lambda>st. P1 st), (0 +
+            npost)-#} [G c z] {#-(\<lambda>st.
+        liftt_conc id l c P2 P1 st), npost-#}"
+    unfolding add_0
+  proof
+    fix c'
+
+    assume Guard : "|#gs#| {#(\<lambda>st. liftt_conc id l c P2 P1 st ), npost#} c'"
+    show "|#gs#| {#(\<lambda>st. P1 st), npost#} ([G c z] @ c')"
+    proof
+      fix m 
+      assume Hpay0 : "P1 (payload m)" and Hcont : "cont m = Inl ([G c z] @ c') "
+
+      show "safe_for gs m npost"
+      proof(cases "(sem_step gs m)")
+        case (Inr bad)
+  
+        then have False using Hcont H0
+          by(auto simp add: sem_step_def)
+  
+        then show ?thesis by auto
+      next
+        case (Inl m')
+
+        have Pres' : "sups_pres (set fs - {seq_sem_l_gen lfts})"
+          using sups_pres_subset[OF Hpres, of "set fs - {seq_sem_l_gen lfts}"] by auto
+
+        obtain fs_sub where Fs_sub : "set fs_sub = set fs - {seq_sem_l_gen lfts}"
+          using finite_list[of "set fs - {seq_sem_l_gen lfts}"]
+          by auto
+
+(* ok, so the idea now is:
+- we know full step (op + control flow) leads to m'
+- dominance over everything but the seq means we can treat it as
+  "op (dominant thing) then seq"
+- we can then unfold these things in order and everything should be ok.
+*)
+
+        have Assoc : 
+             "pcomps (fs_sub @ [seq_sem_l_gen lfts]) =
+              pcomps [pcomps fs_sub, pcomps [seq_sem_l_gen lfts]]"
+        proof(rule pcomps_assoc)
+
+          have "set fs - {seq_sem_l_gen lfts} \<union> set [seq_sem_l_gen lfts] = set fs"
+            using Hseq 
+            by(simp; blast)
+
+          then show "sups_pres (set fs_sub \<union> set [seq_sem_l_gen lfts])"
+            unfolding Fs_sub
+            using Hpres
+            by auto
+        next
+
+          have "set fs_sub \<noteq> {}" using Hnemp unfolding Fs_sub by auto
+
+          then show "fs_sub \<noteq> []" by auto
+        next
+
+          show "[seq_sem_l_gen lfts] \<noteq> []" by simp
+        qed
+
+        have Set_alt : "set (fs_sub @ [seq_sem_l_gen lfts]) = set fs"
+          unfolding set_append Fs_sub
+          using Un_Diff_cancel2 Hseq
+          by auto
+
+        have Gs_alt : "gs = pcomps (fs_sub @ [seq_sem_l_gen lfts])"
+          using pcomps_set_eq[OF Hpres Hseq _ Set_alt, of fs] H0
+          by auto
+
+(* not sure if we need this (ConcX) *)
+(*
+      have ConcX : "liftt_conc id l c P2 P1 (payload m')"
+        sorry
+*)
+(*
+      have (*Hpay1 : "P1 (LOut l c (payload m))" and *) Hpay2 : "payload m \<in> S c" and Hpay3 : "payload m \<in> ok_S"
+        using Hpay lifting_validxDS[OF Valid]
+        unfolding lift_pred_valid_s_def lift_pred_validx_s_def lift_pred_s_def
+        by auto
+*)
+
+(*
+        have Hpay2 : "payload m \<in> S c" and Hpay3 : "payload m \<in> ok_S"
+        using Hpay lifting_validxDS[OF Valid]
+        unfolding lift_pred_valid_s_def lift_pred_validx_s_def lift_pred_s_def
+        by auto
+*)
+
+        have Hpay : "P1 (payload m)"
+          using Hpay0
+          by auto
+
+        then have Hpay_S : "payload m \<in> ok_S"
+          using P1_ok[of "payload m"] by auto
+
+        have Hpay1' : "LOut l (id c) (payload m) = LOut l c (payload m) \<and> P1 (payload m)"
+          using Hpay
+          by simp
+  
+        then have Hpay1 : "\<exists>full. LOut l (id c) full = LOut l c (payload m) \<and> P1 full" using Hpay_S
+          by auto
+
+        have Hpay' : " P2 (\<lambda>st. \<exists>full. LOut l (id c) full = st \<and> P1 full) (f c (LOut l c (payload m)))"
+          using HTSE[OF H ] Hpay1
+          by auto
+
+(* TODO: find a better solution than this awful type annotation hack *)
+        have Seq_pres : 
+          "sups_pres {(seq_sem_l_gen lfts  :: ('b \<Rightarrow> 'b gensyn list md_triv option md_prio \<times>
+            String.literal md_triv option md_prio \<times> 'c
+            \<Rightarrow> 'b gensyn list md_triv option md_prio \<times>
+               String.literal md_triv option md_prio \<times>
+               'c))}"
+          using sups_pres_subset[OF Hpres, of "{seq_sem_l_gen lfts}"] Hseq
+          by(auto)
+
+
+        have Gs_alt' : "gs = pcomps [pcomps fs_sub, seq_sem_l_gen lfts]"
+          using Gs_alt pcomps_singleton[OF Seq_pres, of "[seq_sem_l_gen lfts]"]
+          unfolding Assoc
+          unfolding append.simps H0
+          by auto
+
+        have Hdom' :  "f' \<downharpoonleft> (set fs_sub) c"
+          using Fs_sub Hdom by auto
+
+        have Dominate1 : "pcomps fs_sub c m = f' c m" using dominant_pcomps[OF _ _ Hdom', of g m] Pres' Hnemp Fs_sub
+          by auto
+
+(* YOU ARE HERE. *)
+(* problem: seems like we still need to know something about the validity of the initial state.
+   maybe this is OK, but i worry that it will create problems.
+   the obvious solution is just to throw the validity condition into the pre and post conditions.
+   but let's think about whether that will have unintended consequences.
+ *)
+        obtain pri1 pri2 rest where Msplit :
+          "m = (mdp pri1 (Some (mdt (G c z # c'))), mdp pri2 None, rest)" and Rest : "rest \<in> ok_S"
+          using Gs_alt' Dominate1 Skip Hpay Hcont Hf' Hpay_S
+          by(auto simp add: seq_sem_l_gen_def seq_sem_lifting_gen_def 
+            lift_pred_valid_s_def lift_pred_validx_s_def lift_pred_s_def
+            no_control_lifting_def cont_def
+            schem_lift_defs fst_l_def snd_l_def prio_l_def triv_l_def option_l_def seq_sem_def
+            prod_bsup no_control_l_def
+            split: md_prio.splits prod.splits md_triv.splits option.splits list.split_asm)
+
+        have Rest' : "rest \<in> S c"
+          using lifting_validxDS[OF Valid] Rest by auto
+
+        have LUpd_rest1 :
+          "rest <[ LUpd l c (f c (LOut l c rest)) rest"
+          using lifting_validDI[OF Valid' Rest']
+          by auto
+
+        have LUpd_rest2 : "[^ LUpd l c (f c (LOut l c rest)) rest, rest ^] = LUpd l c (f c (LOut l c rest)) rest"
+          using bsup_base_leq2[OF LUpd_rest1]
+          by simp
+
+        then have LOut_m : "LOut (no_control_lifting l) c (gs c m) = LOut (no_control_lifting l) c (f' c m)"
+          using Gs_alt' Dominate1 Skip Hpay Hcont Hf' Msplit
+          by(auto simp add: seq_sem_l_gen_def seq_sem_lifting_gen_def 
+            lift_pred_valid_s_def lift_pred_s_def
+            no_control_lifting_def cont_def
+            schem_lift_defs fst_l_def snd_l_def prio_l_def triv_l_def option_l_def seq_sem_def
+            prod_bsup no_control_l_def
+            split: md_prio.splits prod.splits md_triv.splits option.splits list.split_asm)
+
+
+(* key sub-result. *)
+
+(* key sub-result. idea here is that no_control_l means we won't overwrite. *)
+        have Cont_final : "cont m' = cont (seq_sem_l_gen lfts c m)"
+          using Hcont Msplit Skip Inl Gs_alt' Dominate1 Hf'
+          by(auto simp add: seq_sem_l_gen_def seq_sem_lifting_gen_def sem_step_def
+            lift_pred_valid_s_def lift_pred_s_def
+            no_control_lifting_def cont_def
+            schem_lift_defs fst_l_def snd_l_def prio_l_def triv_l_def option_l_def seq_sem_def
+            prod_bsup no_control_l_def prio_bsup option_bsup leq_refl
+            split: md_prio.splits prod.splits md_triv.splits option.splits list.split_asm)         
+
+        hence Cont_final' : "cont m' = Inl c'"
+          using Hcont Msplit Skip
+          by(auto simp add: seq_sem_l_gen_def seq_sem_lifting_gen_def sem_step_def
+            lift_pred_valid_s_def lift_pred_s_def
+            no_control_lifting_def cont_def
+            schem_lift_defs fst_l_def snd_l_def prio_l_def triv_l_def option_l_def seq_sem_def
+            prod_bsup no_control_l_def
+            split: md_prio.splits prod.splits md_triv.splits option.splits list.split_asm)
+
+        have Pay_final : "payload m' = LUpd l c (f c (LOut l c (payload m))) (payload m)"
+          using Gs_alt' Dominate1 Skip Hpay Hcont Hf' Msplit Inl LUpd_rest2
+          by(auto simp add: seq_sem_l_gen_def seq_sem_lifting_gen_def sem_step_def
+            lift_pred_valid_s_def lift_pred_s_def
+            no_control_lifting_def cont_def
+            schem_lift_defs fst_l_def snd_l_def prio_l_def triv_l_def option_l_def seq_sem_def
+            prod_bsup no_control_l_def
+            split: md_prio.splits prod.splits md_triv.splits option.splits list.split_asm)
+
+(* YOU ARE HERE *)
+(* TODO: we need to pull out the "ok_S" piece. *)
+        have "payload m' = LUpd l (id c) (f c (LOut l c (payload m)))(payload m) \<and>
+               (P1 (payload m)) \<and>
+               P2 (\<lambda>st. \<exists>full. LOut l (id c) full = st \<and> (P1 full)) (f c (LOut l c (payload m)))"
+          using Hpay' Pay_final Hpay_S Hpay
+          by(auto)
+
+        then have Guard_Hyp : "\<exists>old st_small.
+           payload m' = LUpd l (id c) st_small old \<and>
+           (P1 old) \<and>
+           P2 (\<lambda>st. \<exists>full. LOut l (id c) full = st \<and>
+                            P1 full)
+            st_small"
+          by blast
+
+        have Conc' : "safe_for gs m' npost"
+          using guardediD[OF Guard, of "m'"] Hpay' Cont_final' Guard_Hyp 
+          unfolding Pay_final Cont_final' lift_pred_valid_s_def lift_pred_s_def lift_pred_validx_s_def
+            liftt_conc_def
+          using lifting_validDO[OF Valid'] lifting_validDP[OF Valid'] lifting_validxDP'[OF Valid ]
+          by(cases m; auto)
+
+        have Inl_alt : "sem_step_p gs m m'"
+          using Inl unfolding sem_step_p_eq by simp
+
+        show  "safe_for gs m npost"
+          using safe_for_weaken[OF safe_for_extend[OF Conc' Excp_1[OF Inl_alt]], of npost]
+          by simp
+      qed
+    qed
+  qed
+
+  thus " \<exists>npre.
+          |#gs#| {#-P1, (npre +
+                         npost)-#} [G c
+              z] {#-liftt_conc id l c P2 P1, npost-#}"
+    by blast
+qed
+
 
 (*
 lemma HTS_imp_HT'' :
